asign6.v
@@ -1,3 +1,5 @@
+From Coq Require Import ssreflect ssrfun ssrbool.
+Require Import FunInd.
 Set Implicit Arguments.
 Require Import Coq.Strings.String.
 Require Import Coq.Lists.List.
@@ -18,245 +20,121 @@ Inductive SubContext : ℾ -> ℾ -> Prop :=
 | SubShadow {Γ1 Γ2} Γ' : SubContext Γ1 Γ2 -> SubContext (ShadowEnv Γ1 Γ') (ShadowEnv Γ2 Γ').
 
 Lemma InterpretSubContext {Γ1 Γ2} : SubContext Γ1 Γ2 -> forall {s τ}, s ∷ τ ∈ Γ1 -> s ∷ τ ∈ Γ2.
-  intros H s τ H0.
-  induction H.
-  - apply (H s τ).
-    assumption.
-  - destruct (string_dec s s0) as [-> | neq].
-    + rewrite (InContextUnique H0 (InConsEnv)).
-      constructor.
-    + inversion H0.
-      * congruence.
-      * specialize (IHSubContext inSub).
-        done.
-  - inversion H0.
-    + done.
-    + specialize (IHSubContext inLeft).
-      done.
+  induction 1 => s0 τ0; first done.
+  all:have: forall τ, ContextLookup s0 Γ1 = Some τ -> ContextLookup s0 Γ2 = Some τ
+        by move => ? /InContextP ?; apply/InContextP.
+  all:by move=> IH /InContextP in1; apply/InContextP; move: in1 => /=; program_equiv.
 Qed.
 
-Lemma SubContextRefl Γ : SubContext Γ Γ.
-  enough (forall s τ, s ∷ τ ∈ Γ -> s ∷ τ ∈ Γ).
-  done.
-  trivial.
-Qed.
+Lemma SubContextRefl Γ : SubContext Γ Γ. done. Qed.
 
 Lemma SubContextTrans {Γ1 Γ2 Γ3} : SubContext Γ1 Γ2 -> SubContext Γ2 Γ3 -> SubContext Γ1 Γ3.
-  intros H H0.
-  constructor.
-  intros s τ H1.
-  apply (InterpretSubContext H0).
-  apply (InterpretSubContext H).
-  assumption.
+  by move => /InterpretSubContext ? /InterpretSubContext.
 Qed.
 
 Lemma SubEquiv {Γ1 Γ2} : EquivContext Γ1 Γ2 <-> (SubContext Γ1 Γ2 /\ SubContext Γ2 Γ1).
-  split.
-  - intros H.
-    split.
-    + apply SubIntro.
-      intros s τ H0.
-      rewrite <- (InterpretEquivContext H).
-      assumption.
-    + apply SubIntro.
-      intros s τ H0.
-      rewrite (InterpretEquivContext H).
-      assumption.
-  - intros (ab, ba).
-    apply EquivIntro.
-    intros s τ.
-    split.
-    + exact (InterpretSubContext ab).
-    + exact (InterpretSubContext ba).
+  by move: (@InterpretSubContext) (@InterpretEquivContext Γ1 Γ2).
 Qed.
 
 Notation "a ⊆ b" := (SubContext a b) (at level 1, b at next level).
 
 Lemma SubContextConsRight {Γ1 Γ2} : Γ1 ⊆ Γ2 -> forall x τ, x ∉ Γ1 -> Γ1 ⊆ (ConsEnv x τ Γ2).
-  intros H x τ H0.
-  apply SubIntro.
-  intros s τ0 H1.
-  destruct (string_dec s x) as [-> | neq].
-  - destruct (InContextInverse H1 H0).
-  - pose (InterpretSubContext H H1).
-    done.
+  move=> /InterpretSubContext equiv s τ /InContextPn nin.
+  apply SubIntro => s0 τ0.
+  by case: (string_dec s s0) => [<- /InContextP | neq].
 Qed.
 
-
-Lemma Strengthening {s e} (notInFV : s ∉f e) : forall {Γ τ' τ} (typechecks1 : (ConsEnv s τ' Γ) ⊢ e ∷ τ), Γ ⊢ e ∷ τ.
-  induction notInFV; intros Γ τ' τ'' typechecks1.
-  - inversion typechecks1.
-    subst.
-    constructor.
-    refine (InSubConsEnvInversion _ H1).
-    congruence.
-  - inversion typechecks1.
-    subst.
-    constructor.
-  - inversion typechecks1.
-    subst.
-    constructor.
-    + eapply IHnotInFV1; done.
-    + eapply IHnotInFV2; done.
-  - inversion typechecks1.
-    subst.
-    econstructor.
-    + eapply IHnotInFV1; done.
-    + eapply IHnotInFV2; done.
-  - inversion typechecks1.
-    subst.
-    constructor.
-    assumption.
-    eapply IHnotInFV.
-    enough (EquivContext (ConsEnv x τ (ConsEnv f (τ → τ'0) (ConsEnv s τ' Γ)))
-                         (ConsEnv s τ' (ConsEnv x τ (ConsEnv f (τ → τ'0) Γ)))).
-    exact (EquivContextAlsoTypechecks type1 H).
-    pose (EquivContextReorder (EquivContextRefl (ConsEnv f (τ → τ'0) Γ)) notX τ τ').
-    pose (EquivCons x τ (EquivContextReorder (EquivContextRefl Γ) notF (AbsType τ τ'0) τ')).
-    exact (EquivContextTrans e0 e).
-  - inversion typechecks1.
-    subst.
-    constructor.
-    assumption.
-    enough (EquivContext (ConsEnv x τ (ConsEnv f (τ → τ'0) (ConsEnv x τ' Γ))) (ConsEnv x τ (ConsEnv f (τ → τ'0) Γ))).
-    exact (EquivContextAlsoTypechecks type1 H).
-    pose (EquivCons x τ (EquivContextReorder (EquivContextRefl Γ) nefx (AbsType τ τ'0) τ')).
-    pose (EquivContextDoubleElim (ConsEnv f (τ → τ'0) Γ) x τ τ').
-    exact (EquivContextTrans e e0).
-  - inversion typechecks1.
-    subst.
-    constructor.
-    assumption.
-    enough (EquivContext (ConsEnv x τ (ConsEnv f (τ → τ'0) (ConsEnv f τ' Γ))) (ConsEnv x τ (ConsEnv f (τ → τ'0) Γ))).
-    exact (EquivContextAlsoTypechecks type1 H).
-    exact (EquivCons x τ (EquivContextDoubleElim Γ f (AbsType τ τ'0) τ')).
+Lemma Weakening {Γ e τ} (typchecks1 : Γ ⊢ e ∷ τ) : forall {Γ'}, Γ ⊆ Γ' -> Γ' ⊢ e ∷ τ.
+  by induction typchecks1 => // Γ'' /InterpretSubContext.
 Qed.
 
-Lemma Weakening {Γ e τ} (typchecks1 : Γ ⊢ e ∷ τ) :
-  forall {Γ'}, Γ ⊆ Γ' -> Γ' ⊢ e ∷ τ.
-Proof with done.
-  induction typchecks1; intros Γ'' Γ''sub.
-  - done.
-  - refine (VSE (InterpretSubContext Γ''sub _))...
-  - refine (ASE (IHtypchecks1_1 _ _)
-                (IHtypchecks1_2 _ _))...
-  - refine (PSE (IHtypchecks1_1 _ _)
-                (IHtypchecks1_2 _ _))...
-  - specialize (IHtypchecks1 (ConsEnv x τ (ConsEnv f (τ → τ') Γ''))
-                             (SubCons x τ (SubCons f (τ → τ') Γ''sub)))...
-Qed.
+Ltac weakening := apply/Weakening/(SubContextConsRight (SubContextRefl _)).
 
 Lemma OtherWeakening {s e} (sNotIn : s ∉f e) : forall {Γ τ} (typechecks1 : Γ ⊢ e ∷ τ) {τ'}, (ConsEnv s τ' Γ) ⊢ e ∷ τ.
-Proof with done.
-  induction sNotIn; intros Γ τ'' typechecks1 τ'; inv typechecks1; econstructor; subst.
-  - refine (InSubConsEnv _ _)...
-  - eapply IHsNotIn1...
-  - eapply IHsNotIn2...
-  - eapply IHsNotIn1...
-  - eapply IHsNotIn2...
-  - assumption.
-  - specialize (IHsNotIn (ConsEnv x τ (ConsEnv f (τ → τ'0) Γ)) τ'0 type1 τ').
-    apply (EquivContextAlsoTypechecks IHsNotIn).
-    pose (EquivContextReorder (EquivContextRefl (ConsEnv f (τ → τ'0) Γ)) notX τ τ').
-    pose (EquivCons x τ (EquivContextReorder (EquivContextRefl Γ) notF (AbsType τ τ'0) τ')).
-    exact (EquivContextSymm (EquivContextTrans e0 e)).
-  - assumption.
-  - refine (EquivContextAlsoTypechecks type1 _).
-    pose (EquivCons x τ (EquivContextReorder (EquivContextRefl Γ) nefx (AbsType τ τ'0) τ')).
-    pose (EquivContextDoubleElim (ConsEnv f (τ → τ'0) Γ) x τ τ').
-    exact (EquivContextSymm (EquivContextTrans e e0)).
-  - assumption.
-  - refine (EquivContextAlsoTypechecks type1 _).
-    exact (EquivContextSymm (EquivCons x τ (EquivContextDoubleElim Γ f (AbsType τ τ'0) τ'))).
+  induction sNotIn; intros Γ τ'' typechecks1 τ'; inv typechecks1; econstructor => //=.
+  - specialize (IHsNotIn (ConsEnv x τarg (ConsEnv f (τarg → τret) Γ)) τret type1 τ').
+    apply/(EquivContextAlsoTypechecks IHsNotIn)/EquivContextP => s0 /=.
+    by program_equiv.
+  - apply/(EquivContextAlsoTypechecks type1)/EquivContextP => s0 /=.
+    by program_equiv.
+  - apply/(EquivContextAlsoTypechecks type1)/EquivContextP => s0 /=.
+    by program_equiv.
 Qed.
 
 Reserved Notation "a ≡ b % c" (at level 1, b at next level).
 
 Inductive ContextCongruenceModuloS : ℾ -> ℾ -> string -> Prop :=
 | CongModIntro Γ1 Γ2 s :
-    (forall s' τ, (s=s') \/ (s' ∷ τ ∈ Γ1 <-> s' ∷ τ ∈ Γ2)) ->
+    (forall s', (s=s') \/ (forall τ, s' ∷ τ ∈ Γ1 <-> s' ∷ τ ∈ Γ2)) ->
     (Γ1 ≡ Γ2 % s)
 | CongModCons {Γ1 Γ2 s s' τ} : Γ1 ≡ Γ2 % s -> (ConsEnv s' τ Γ1) ≡ (ConsEnv s' τ Γ2) % s
 | CongModShad {Γ1 Γ2 Γ' s} : Γ1 ≡ Γ2 % s -> (ShadowEnv Γ1 Γ') ≡ (ShadowEnv Γ2 Γ') % s
 where "a ≡ b % c" := (ContextCongruenceModuloS a b c).
 
-Lemma CongModRefl Γ s : Γ ≡ Γ % s.
-  apply CongModIntro.
-  intros s' τ.
-  right.
-  reflexivity.
+Lemma InEquivToNotInEquiv {s Γ1 Γ2} : (forall τ, s ∷ τ ∈ Γ1 <-> s ∷ τ ∈ Γ2) -> (s ∉ Γ1 <-> s ∉ Γ2).
+  move=> eq1.
+  split => nin1.
+  case (InContextOptions Γ2 s) => //=.
+  move=> [? /eq1/InContextInverse] //=.
+  case (InContextOptions Γ1 s) => //=.
+  move=> [? /eq1/InContextInverse] //=.
 Qed.
 
 Lemma InterpretCongMod' {Γ1 Γ2 s}
-  : Γ1 ≡ Γ2 % s -> forall s' τ, (s=s') \/ (s' ∷ τ ∈ Γ1 <-> s' ∷ τ ∈ Γ2).
-  intros H s' τ.
-  induction H.
-  - exact (H s' τ).
-  - decompose [or] IHContextCongruenceModuloS.
-    + done.
+  : Γ1 ≡ Γ2 % s -> forall s', (s=s') \/ (forall τ, s' ∷ τ ∈ Γ1 <-> s' ∷ τ ∈ Γ2).
+  intros H s'.
+  induction H; first done.
+  - decompose [or] IHContextCongruenceModuloS; first done.
+    right; split; inversion 1; done.
+  - decompose [or] IHContextCongruenceModuloS; first done.
+    right; split; inversion 1; done.
+Qed.
+
+Lemma CongModP {Γ1 Γ2 s} :
+  Γ1 ≡ Γ2 % s <-> (forall s0, (string_dec s s0)||(OptionLType_dec (ContextLookup s0 Γ1) (ContextLookup s0 Γ2))).
+  split.
+  - move/InterpretCongMod' => cong s0.
+    apply/orP.
+    case/(_ s0): cong.
+    + left; exact/sumboolP.
     + right.
-      destruct H0.
-      split; inversion 1; done.
-  - decompose [or] IHContextCongruenceModuloS.
-    + done.
-    + right.
-      destruct H0.
-      split; inversion 1; done.
+      apply/sumboolP.
+      set o := (ContextLookup _ Γ2).
+      case E : o.
+      * apply/InContextP/b; move/InContextP: E; done.
+      * move/InEquivToNotInEquiv in b.
+        apply/InContextPn/b; move/InContextPn: E; done.
+  - move=> equiv.
+    apply CongModIntro.
+    move=> s0; case/(_ s0)/orP : equiv.
+    + move/sumboolP; done.
+    + move/sumboolP => equiv.
+      right => τ; split => /InContextP eq; exact/InContextP.
 Qed.
 
 Lemma InterpretCongMod {Γ1 Γ2 s}
-  : Γ1 ≡ Γ2 % s -> forall {s' τ}, s<>s' -> (s' ∷ τ ∈ Γ1 <-> s' ∷ τ ∈ Γ2).
+  : Γ1 ≡ Γ2 % s -> forall {s'}, s<>s' -> (forall τ, s' ∷ τ ∈ Γ1 <-> s' ∷ τ ∈ Γ2).
   intros H s' τ H0.
-  destruct (InterpretCongMod' H s' τ); done.
+  edestruct (InterpretCongMod' H s'); done.
+Qed.
+
+Lemma CongModRefl Γ s : Γ ≡ Γ % s.
+  done.
 Qed.
 
 Lemma CongModSymm {Γ1 Γ2 s} : Γ1 ≡ Γ2 % s -> Γ2 ≡ Γ1 % s.
-  intros H.
-  eapply CongModIntro.
-  intros s' τ.
-  destruct (string_dec s s') as [-> | neq].
-  - done.
-  - right.
-    symmetry.
-    apply (InterpretCongMod H neq).
+  by move=> /InterpretCongMod' cong; apply/CongModIntro => s0; move/(_ s0): cong => [|].
 Qed.
 
-Lemma CongModToEquiv {Γ1 Γ2 s} : Γ1 ≡ Γ2 % s -> forall τ, (EquivContext (ConsEnv s τ Γ1) (ConsEnv s τ Γ2)).
-  intros H τ.
-  eapply EquivIntro.
-  intros s0 τ0.
-  epose (InterpretCongMod' H).
-  - destruct (string_dec s s0) as [-> | neq].
-    + split; intros H'; inversion H'; done.
-    + destruct (o s0 τ0) as [-> | equiv].
-      contradiction.
-      split; intros H'; inversion H'; done.
+Lemma CongModToEquiv {Γ1 Γ2 s} (cong: Γ1 ≡ Γ2 % s) τ : (EquivContext (ConsEnv s τ Γ1) (ConsEnv s τ Γ2)).
+  apply/EquivContextP => s0 /=; case (string_dec s0 s) => //= ne.
+  case/CongModP/(_ s0)/orP: cong => /sumboolP //=.
 Qed.
 
 Lemma CongModConsLeft {x τ Γ1 Γ2} : Γ1 ≡ Γ2 % x -> (ConsEnv x τ Γ1) ≡ Γ2 % x.
-  intros H.
-  eapply CongModIntro.
-  intros s' τ0.
-  destruct (string_dec s' x) as [-> | neq].
-  - done.
-  - right.
-    split.
-    + intros H0.
-      pose (InSubConsEnvInversion neq H0).
-      eapply InterpretCongMod.
-      eapply CongModSymm.
-      exact H.
-      congruence.
-      eapply InSubConsEnvInversion.
-      exact neq.
-      exact H0.
-    + intros H0.
-      eapply InSubConsEnv.
-      done.
-      enough (x <> s').
-      rewrite (InterpretCongMod H H1).
-      done.
-      congruence.
+  move => /CongModP cong; apply/CongModP => s0; apply/orP.
+  case/(_ s0)/orP: cong => //= /sumboolP eq.
+  case (string_dec s0 x);[left | right]; exact/sumboolP.
 Qed.
 
 Lemma Substitution {e1 Γ1 τ1} (typechks1 : Γ1 ⊢ e1 ∷ τ1) : forall e2 e3 Γ2 τ2 s,
@@ -265,238 +143,117 @@ Lemma Substitution {e1 Γ1 τ1} (typechks1 : Γ1 ⊢ e1 ∷ τ1) : forall e2 e3 
   Γ1 ≡ Γ2 % s ->
   [e2 / s] e1 = e3 ->
   Γ2 ⊢ e3 ∷ τ1.
-Proof with done.
-  intros e2 e3 Γ2 τ2 s H H0 H1 H2.
-  dependent induction typechks1. 
-  - inversion H2...
-  - inversion H3.
-    subst.
-    rewrite (InContextUnique H H0)...
-    rewrite (InterpretCongMod H2 neq) in H...
-  - inversion H2.
-    subst.
-    constructor.
-    + eapply IHtypechks1_1.
-      exact H.
-      exact H0.
-      exact H1.
-      exact LeftAddCAS.
-    + eapply IHtypechks1_2.
-      exact H.
-      exact H0.
-      exact H1.
-      exact RightAddCAS.
-  - inversion H2.
-    subst.
-    eapply PSE.
-    + eapply IHtypechks1_1.
-      exact H.
-      exact H0.
-      exact H1.
-      exact LeftAppCAS.
-    + eapply IHtypechks1_2.
-      exact H.
-      exact H0.
-      exact H1.
-      exact RightAppCAS.
-  - inversion H2.
-    subst.
-    + eapply BSE.
-      assumption.
-      eapply IHtypechks1.
-      * exact (InSubConsEnv notX (InSubConsEnv notF H)).
-      * eapply (OtherWeakening _).
-        eapply (OtherWeakening _).
-        eassumption.
-      * exact (CongModCons (CongModCons H1)).
-      * assumption.
-    + subst.
-      eapply BSE.
-      assumption.
-      pose (EquivCons x τ (CongModToEquiv H1 (τ → τ'))).
-      refine (EquivContextAlsoTypechecks _ _).
-      exact typechks1.
-      exact e.
-    + subst.
-      eapply BSE.
-      assumption.
-      pose (@CongModCons _ _ _ f (τ → τ') H1).
-      pose (CongModToEquiv c τ).
-      refine (EquivContextAlsoTypechecks _ _).
-      exact typechks1.
-      exact e.
-      Unshelve.
-      assumption.
-      assumption.
+  elim: typechks1; intros; match goal with | H : [ _ / _ ] _ = _ |- _ => inversion H end; subst.
+  - done.
+  - move/InContextP in H; move/InContextP in H0; done.
+  - move/(InterpretCongMod H2 neq) in H; done.
+  - done.
+  - done.
+  - have: s ∷ τ2 ∈ (ConsEnv x τarg (ConsEnv f (τarg → τret) Γ)) by done.
+    have: (ConsEnv x τarg (ConsEnv f (τarg → τret) Γ2)) ⊢ e2 ∷ τ2 by exact/OtherWeakening/OtherWeakening.
+    have: (ConsEnv x τarg (ConsEnv f (τarg → τret) Γ)) ≡ (ConsEnv x τarg (ConsEnv f (τarg → τret) Γ2)) % s
+      by exact/CongModCons/CongModCons.
+    done.
+  - have: f ∷ (τarg → τret) ∈ (ConsEnv x τarg (ConsEnv f (τarg → τret) Γ)) by done.
+    have: (EquivContext (ConsEnv x τarg (ConsEnv f (τarg → τret) Γ)) (ConsEnv x τarg (ConsEnv f (τarg → τret) Γ2)))
+      by exact/EquivCons/CongModToEquiv.
+    by move/EquivContextAlsoTypechecks.
+  - have: x ∷ τarg ∈ (ConsEnv x τarg (ConsEnv f (τarg → τret) Γ)) by done.
+    have: (EquivContext (ConsEnv x τarg (ConsEnv f (τarg → τret) Γ)) (ConsEnv x τarg (ConsEnv f (τarg → τret) Γ2)))
+      by exact/CongModToEquiv/CongModCons.
+    by move/EquivContextAlsoTypechecks.
 Qed.
 
 Lemma CannonicalForms {e τ} :
   NullEnv ⊢ e ∷ τ -> (𝕍 e) ->
   match τ with
   | NatType => exists n, e = (NatExpr n)
-  | (AbsType τ1 τ2) => exists f x body, f<>x /\ (e = (AbsExpr f x τ1 body))
+  | (AbsType τ1 τ2) => exists f x body, f<>x /\ (e = (AbsExpr f x τ1 τ2 body))
   end.
-  intros H H0.
-  destruct H.
-  - exists n; done.
-  - inversion H0.
-  - inversion H0.
-  - inversion H0.
-  - exists f.
-    exists x.
-    exists body.
-    done.
+  by case.
 Qed.
 
-Lemma TypedEvalContextInversion {Γ E τ0 τ} (Etype : Γ ⊢ E [τ0] ∷ τ)
-  : exists x e, x ∉ Γ /\ EvaluationContextFillsTo E x e /\ (ConsEnv x τ0 Γ) ⊢ e ∷ τ.
-  destruct Etype.
-  - destruct (ContextFinite Γ).
-    exists x.
-    exists x.
-    done.
-  - exists x.
-    exists (AddExpr e1 e2).
-    epose (Weakening H (SubContextConsRight (SubContextRefl Γ) τ H0)).
-    done.
-  - exists x.
-    exists (AddExpr n e).
-    done.
-  - exists x.
-    exists (AppExpr e1 e2).
-    epose (Weakening H (SubContextConsRight (SubContextRefl Γ) τ H0)).
-    done.
-  - exists x.
-    exists (AppExpr (AbsExpr fn arg τarg body) e).
-    epose (Weakening H (SubContextConsRight (SubContextRefl Γ) τ H0)).
-    done.
+Lemma TypedEvalContextInversion {Γ E τ0 τ} : Γ ⊢ E {τ0} ∷ τ -> exists x, x ∉ Γ /\ (ConsEnv x τ0 Γ) ⊢ E[x] ∷ τ.
+  destruct 1; simpl.
+  - destruct (ContextFinite Γ) => //=.
+  - by have: (ConsEnv x τ Γ) ⊢ e ∷ ℕ by weakening.
+  - done.
+  - by have: (ConsEnv x τ Γ) ⊢ e ∷ τarg by weakening.
+  - by have: (ConsEnv x τ Γ) ⊢ (AbsExpr fn arg τarg τret body) ∷ (τarg → τret) by weakening.
 Qed.
 
-Lemma DecompositionOfTypes {E} : forall {e0 e1 Γ τ},
-    EvaluationContextFillsTo E e0 e1 -> Γ ⊢ e1 ∷ τ -> exists τ1, Γ ⊢ e0 ∷ τ1 /\ Γ ⊢ E [τ1] ∷ τ.
-  induction E; intros e0 e1 Γ τ' H H0.
-  all:inversion H; subst.
-  exists τ'; done.
-  all:inversion H0; subst.
-  - destruct (IHE e0 e1' Γ NatType subFills type1) as (τ1, (typ1, typ2)).
-    exists τ1.
-    destruct (TypedEvalContextInversion typ2) as (x, (e2, (notIn, (fills, typ3)))).
-    done.
-  - destruct (IHE e0 e2' Γ NatType subFills type2) as (τ1, (typ1, typ2)).
-    exists τ1.
-    destruct (TypedEvalContextInversion typ2) as (x, (e2, (notIn, (fills, typ3)))).
-    done.
-  - destruct (IHE e0 e1' Γ (AbsType τ1 τ') subFills type1) as (τ2, (typ1, typ2)).
-    exists τ2.
-    destruct (TypedEvalContextInversion typ2) as (x, (e2, (notIn, (fills, typ3)))).
-    done.
-  - inversion type1.
-    destruct (IHE e0 e2' Γ τ1 subFills type2) as (τ2, (typ1, typ2)).
-    exists τ2.
-    destruct (TypedEvalContextInversion typ2) as (s, (e2, (notIn, (fills, typ3)))).
-    done.
+Lemma DecompositionOfTypes E : forall Γ e0 τ, Γ ⊢ E[e0] ∷ τ -> exists τ1, Γ ⊢ e0 ∷ τ1 /\ Γ ⊢ E {τ1} ∷ τ.
+  induction E; intros; simpl in *; first done.
+  all:inversion H.
+  - by move/IHE: type1 => [τx [? b]]; move:(TypedEvalContextInversion b) => [? [? ?]].
+  - by move/IHE: type2 => [τx [? b]]; move:(TypedEvalContextInversion b) => [? [? ?]].
+  - by move/IHE: type1 => [τx [? b]]; move:(TypedEvalContextInversion b) => [? [? ?]].
+  - by inversion type1; move/IHE: type2 => [τx [? b]]; move:(TypedEvalContextInversion b) => [? [? ?]].
 Qed.
 
 Definition CanStep e := exists e', e ⥛ e'.
 Definition NotStuck e := 𝕍 e \/ (CanStep e).
 
+Lemma Progressβ : forall {e τ} (ety: NullEnv ⊢ e ∷ τ), (𝕍 e) \/ (exists E e0 e1, e = E[e0] /\ e0 ⥛β e1).
+  elim => //=.
+  - move=> x τ; inversion 1; inversion H1.
+  - move => e1 H1 e2 H2 τ; inversion 1; right.
+    move/(_ NatType type1): H1 => [/(CannonicalForms type1) v1| [E1 [e11 [e12 [-> step1]]]]].
+    all:move/(_ NatType type2): H2 => [/(CannonicalForms type2) v2| [E2 [e21 [e22 [-> step2]]]]].
+    + move: v1 => [n1 ->]; move: v2 => [n2 ->]; exists Hole; exists (AddExpr n1 n2); exists (NatExpr (n1 + n2)); done.
+    + move: v1 => [n1 ->]; exists (EvalContextRAdd n1 E2); exists e21; exists e22; done.
+    + move: v2 => [n2 ->]; exists (EvalContextLAdd E1 n2); exists e11; exists e12; done.
+    + exists (EvalContextLAdd E1 (E2 [e21])); exists e11; exists e12; done.
+  - move => e1 H1 e2 H2 τ; inversion 1; right.
+    move/(_ (AbsType τ1 τ) type1): H1 => [/(CannonicalForms type1) v1| [E1 [e11 [e12 [-> step1]]]]].
+    all:move/(_ τ1 type2): H2 => [v2| [E2 [e21 [e22 [-> step2]]]]].
+    + move: v1 => [f [x [body [nefx ->]]]].
+      exists Hole.
+      exists (AppExpr (AbsExpr f x τ1 τ body) e2); simpl.
+      move:(@CASAlways e2 x body (AlwaysSafeToSubInto _ _)) => [body' eq].
+      move:(@CASAlways (AbsExpr f x τ1 τ body) f body' (AlwaysSafeToSubInto _ _)) => [body'' eq'].
+      done.
+    + move: v1 => [f [x [body [nefx ->]]]]; exists (EvalContextRApp f x τ1 τ body E2); exists e21; exists e22; done.
+    + exists (EvalContextLApp E1 e2); exists e11; exists e12; done.
+    + exists (EvalContextLApp E1 (E2 [e21])); exists e11; exists e12; done.
+Qed.
+
 Lemma Progress {e} : forall {τ} (etyp: NullEnv ⊢ e ∷ τ), (NotStuck e).
-  induction e.
-  - intros; subst.
-    inversion etyp.
-    inversion H1.
-  - left; now constructor.
-  - intros τ etyp.
-    inversion etyp.
-    right.
-    subst.
-    specialize (IHe1 _ type1).
-    specialize (IHe2 _ type2).
-    destruct IHe1 as [ ve1 | se1 ].
-    + destruct (CannonicalForms type1 ve1).
-      subst.
-      destruct IHe2 as [ ve2 | se2 ].
-      * destruct (CannonicalForms type2 ve2).
-        exists (NatExpr (x + x0)).
-        done.
-      * inversion se2.
-        inversion H.
-        done.
-    + inversion se1.
-      inversion H.
-      exists (AddExpr x e2).
-      done.
-  - done.
-  - intros τ etyp.
-    inversion etyp.
-    subst.
-    specialize (IHe1 _ type1).
-    specialize (IHe2 _ type2).
-    right.
-    destruct IHe1 as [ ve1 | se1 ].
-    + destruct (CannonicalForms type1 ve1) as (f1, (x1, (body1, (ne1, eq1)))).
-      subst.
-      * inversion type1.
-        subst.
-        destruct IHe2 as [ ve2 | se2 ].
-        -- destruct (@CASAlways e2 x1 body1) as (body2, cas1).
-           apply AlwaysSafeToSubInto.
-           destruct (@CASAlways (AbsExpr f1 x1 τ1 body1) f1 body2) as (body3, cas2).
-           apply AlwaysSafeToSubInto.
-           exists body3.
-           done.
-        -- inversion se2.
-           inversion H.
-           subst.
-           exists (AppExpr (AbsExpr f1 x1 τ1 body1) x).
-           done.
-    + inversion se1.
-      inversion H.
-      exists (AppExpr x e2).
-      done.
+  by move=> τ /Progressβ; move=> [v | [E [e0 [e1 [-> bstep]]]]].
 Qed.
 
 Lemma βPreservation {e e'} (estep : e ⥛β e') : forall τ (etyp : NullEnv ⊢ e ∷ τ),  NullEnv ⊢ e' ∷ τ.
-  induction estep; intros τ0 etyp; inversion etyp.
+  induction estep; intros τ0 etyp; inversion etyp; first done.
+  subst.
+  inversion type1.
+  subst.
+  apply/Substitution.
+  - apply/Substitution.
+    + exact type0.
+    + done.
+    + have: (NullEnv ⊆ (ConsEnv f (τ1 → τ0) NullEnv)) by apply/(SubContextConsRight (SubContextRefl _))/NotInNullEnv.
+      move=> sub; exact/Weakening.
+    + apply/CongModConsLeft/CongModRefl.
+    + done.
+  - apply/InConsEnv.
+  - exact type1.
+  - apply/CongModConsLeft/CongModRefl.
   - done.
-  - subst.
-    inversion type1.
-    subst.
-    eapply Substitution.
-    + eapply Substitution.
-      * exact type0.
-      * apply InConsEnv.
-      * eapply Weakening.
-        exact type2.
-        eapply SubContextConsRight.
-        apply SubContextRefl.
-        apply (@NotInNullEnv f).
-      * eapply CongModConsLeft.
-        apply CongModRefl.
-      * exact CASx.
-    + apply InConsEnv.
-    + exact type1.
-    + eapply CongModConsLeft.
-      apply CongModRefl.
-    + exact CASf.
 Qed.
 
 Lemma Preservation {e e'} (estep : e ⥛ e') : forall τ (etyp : NullEnv ⊢ e ∷ τ),  NullEnv ⊢ e' ∷ τ.
   intros τ etyp.
   inversion estep.
   subst.
-  destruct (DecompositionOfTypes fillse1 etyp) as (τn, (typee1, ?)).
-  pose (typee2 := βPreservation betaStep typee1).
-  eapply InterpretTypedEvalContext.
-  exact H.
-  exact typee2.
-  exact fillse2.
+  move: (DecompositionOfTypes E e1 etyp) => [τn [typee1 ?]].
+  move: (βPreservation betaStep typee1) => etyp1.
+  exact/InterpretTypedEvalContext.
 Qed.
 
 Lemma Safety {e τ} (etyp : NullEnv ⊢ e ∷ τ) {e'} (estep : e ⥛* e') : (NotStuck e').
   induction estep.
-  - now apply (Progress etyp).
-  - apply (IHestep (Preservation ess etyp)).
+  - exact/Progress.
+  - exact/IHestep/Preservation.
 Qed.
 
 
