dynamic_semantics.v
@@ -12,6 +12,7 @@ decide equality.
 - apply string_dec.
 - decide equality.
 - decide equality.
+- decide equality.
 - apply string_dec.
 - apply string_dec.
 Qed.
@@ -21,18 +22,15 @@ Reserved Notation "a ⥛β b" (at level 1, no associativity).
 
 Inductive SmallStepsBeta : 𝔼 -> 𝔼 -> Prop :=
 | ASSβ n1 n2 : ((NatExpr n1) + (NatExpr n2)) ⥛β (NatExpr (n1 + n2))
-| PSSβ f x τ body {e} (v : 𝕍 e) {body' body''}
+| PSSβ f x τarg τret body {e} (v : 𝕍 e) {body' body''}
        (CASx : [ e / x ] body = body')
-       (CASf : [ (AbsExpr f x τ body) / f ] body' = body'')
-  : (AppExpr (AbsExpr f x τ body) e) ⥛β body''
+       (CASf : [ (AbsExpr f x τarg τret body) / f ] body' = body'')
+  : (AppExpr (AbsExpr f x τarg τret body) e) ⥛β body''
 where "a ⥛β b" := (SmallStepsBeta a b).
 
 Inductive SmallSteps : 𝔼 -> 𝔼 -> Prop :=
-| ECSS {E e1 e1' e2 e2'}
-       (fillse1 : EvaluationContextFillsTo E e1 e1')
-       (fillse2 : EvaluationContextFillsTo E e2 e2')
-       (betaStep : e1 ⥛β e2)
-  : e1' ⥛ e2'
+| ECSS {E e1 e2} (betaStep : e1 ⥛β e2)
+  : E[e1] ⥛ E[e2]
 where "a ⥛ b" := (SmallSteps a b).
 
 Reserved Notation "a ⥛* b" (at level 1, no associativity).
