lang.v
@@ -13,31 +13,36 @@ Lemma LType_dec : forall (τ1 τ2 : LType), {τ1=τ2} + {τ1 <> τ2}.
   decide equality.
 Defined.
 
+Bind Scope LType_scope with LType.
+Notation "'ℕ'" := NatType : LType_scope.
+Notation "a → b" := (AbsType a b) (at level 50, left associativity) : LType_scope.
+
 Inductive Expression : Set :=
 | VarExpr (x : string) : Expression
 | NatExpr (n : nat) : Expression
 | AddExpr (e1 e2 : Expression) : Expression
-| AbsExpr (f x : string) (τ : LType) (body : Expression) : Expression
+| AbsExpr (f x : string) (τarg τret : LType) (body : Expression) : Expression
 | AppExpr (e1 e2 : Expression) : Expression.
 
 Coercion VarExpr : string >-> Expression.
 Coercion NatExpr : nat >-> Expression.
 Bind Scope Expression_scope with Expression.
 Arguments AddExpr (e1 e2)%Expression_scope.
+Arguments AbsExpr (f x)%string_scope (τarg τret)%LType_scope body%Expression_scope.
 Notation "a + b" := (AddExpr a b) : Expression_scope.
 
 Inductive LValue : Expression -> Prop :=
 | NatValue n: LValue (NatExpr n)
-| AbsValue (f x : string) (τ : LType) (body : Expression) : LValue (AbsExpr f x τ body).
+| AbsValue (f x : string) (τarg τret : LType) (body : Expression) : LValue (AbsExpr f x τarg τret body).
 
 Inductive EvaluationContext : Set :=
 | Hole : EvaluationContext
 | EvalContextLAdd (E : EvaluationContext) (e : Expression) : EvaluationContext
 | EvalContextRAdd (n : nat) (E : EvaluationContext) : EvaluationContext
 | EvalContextLApp (E : EvaluationContext) (e : Expression) : EvaluationContext
-| EvalContextRApp (f x : string) (τ : LType) (body : Expression) (E : EvaluationContext) : EvaluationContext.
+| EvalContextRApp (f x : string) (τarg τret : LType) (body : Expression) (E : EvaluationContext) : EvaluationContext.
 
-Reserved Notation "E [ e ]" (at level 1, e at next level).
+Reserved Notation "E [ e ]" (at level 0, e at next level).
 
 Fixpoint FillEvaluationContext E e :=
   match E with
@@ -45,17 +50,13 @@ Fixpoint FillEvaluationContext E e :=
   | EvalContextLAdd E0 e0 => (AddExpr E0[e] e0)
   | EvalContextRAdd n E0 => (AddExpr n E0[e])
   | EvalContextLApp E0 e0 => (AppExpr E0[e] e0)
-  | EvalContextRApp f x τ body E0 =>
-    (AppExpr (AbsExpr f x τ body) E0[e])
+  | EvalContextRApp f x τarg τbody body E0 =>
+    (AppExpr (AbsExpr f x τarg τbody body) E0[e])
   end
 where "E [ e ]" := (FillEvaluationContext E e).
 
 Functional Scheme FillEvaluationContext_ind
   := Induction for FillEvaluationContext Sort Set.
-
-Bind Scope LType_scope with LType.
-Notation "'ℕ'" := NatType : LType_scope.
-Notation "a → b" := (AbsType a b) (at level 50, left associativity) : LType_scope.
 
 Notation 𝔼 := Expression.
 Notation 𝕋 := LType.
